New step relation implemented

rupicola/stlc/STLC.fst
@@ -226,87 +226,118 @@ let subst_beta (v e:exp) :
   lem_subst_freevars_closes_exp (sub_beta v) e 0;
   subst (sub_beta v) e
 
-val step : closed_exp -> option closed_exp
-let rec step e =
-  match e with
-  | EApp e1 e2 -> begin
-      match step e1 with (** PO-app1 **)
-      | Some e1' -> Some (EApp e1' e2)
-      | None     -> begin
-          match step e2 with (** PO-app2 **)
-          | Some e2' -> Some (EApp e1 e2')
-          | None     -> begin
-            match e1 with (** PO-app3 **)
-            | ELam e' -> begin
-              Some (subst_beta e2 e')
-            end
-            | _ -> None
-          end
-      end
-  end
-  | EIf e1 e2 e3 -> begin
-    match step e1 with
-    | Some e1' -> Some (EIf e1' e2 e3)
-    | None -> begin
-      match e1 with
-      | ETrue -> Some e2
-      | EFalse -> Some e3
-      | _ -> None
-    end
-  end
-  | EPair e1 e2 -> begin
-    match step e1 with
-    | Some e1' -> Some (EPair e1' e2)
-    | None -> begin
-      match step e2 with
-      | Some e2' -> Some (EPair e1 e2')
-      | None -> None
-    end
-  end
-  | EFst e' -> begin
-    match step e' with
-    | Some e'' -> Some (EFst e'')
-    | None -> begin
-      match e' with
-      | EPair e1 _ -> Some e1
-      | _ -> None
-    end
-  end
-  | ESnd e' -> begin
-    match step e' with
-    | Some e'' -> Some (ESnd e'')
-    | None -> begin
-      match e' with
-      | EPair _ e2 -> Some e2
-      | _ -> None
-    end
-  end
-  | _ -> None
-
+noeq
+type step : closed_exp -> closed_exp -> Type =
+  | AppLeft :
+    #e1:closed_exp ->
+    e2:closed_exp ->
+    #e1':closed_exp ->
+    hst:step e1 e1' ->
+    step (EApp e1 e2) (EApp e1' e2)
+  | AppRight :
+    e1:closed_exp ->
+    #e2:closed_exp ->
+    #e2':closed_exp ->
+    is_value e1 ->
+    hst:step e2 e2' ->
+    step (EApp e1 e2) (EApp e1 e2')
+  | Beta :
+    e11:exp{is_closed (ELam e11)} ->
+    e2:value ->
+    step (EApp (ELam e11) e2) (subst_beta e2 e11)
+  | IfCond :
+    #e1:closed_exp ->
+    e2:closed_exp ->
+    e3:closed_exp ->
+    #e1':closed_exp ->
+    hst:step e1 e1' ->
+    step (EIf e1 e2 e3) (EIf e1' e2 e3)
+  | IfTrue :
+    e2:closed_exp ->
+    e3:closed_exp ->
+    step (EIf ETrue e2 e3) e2
+  | IfFalse :
+    e2:closed_exp ->
+    e3:closed_exp ->
+    step (EIf EFalse e2 e3) e3
+  | PairLeft :
+    #e1:closed_exp ->
+    e2:closed_exp ->
+    #e1':closed_exp ->
+    hst:step e1 e1' ->
+    step (EPair e1 e2) (EPair e1' e2)
+  | PairRight :
+    e1:closed_exp ->
+    #e2:closed_exp ->
+    #e2':closed_exp ->
+    is_value e1 ->
+    hst:step e2 e2' ->
+    step (EPair e1 e2) (EPair e1 e2')
+  | FstPair :
+    #e':closed_exp ->
+    #e'':closed_exp ->
+    hst:step e' e'' ->
+    step (EFst e') (EFst e'')
+  | FstPairReturn :
+    #e1:closed_exp ->
+    #e2:closed_exp ->
+    is_value (EPair e1 e2) ->
+    step (EFst (EPair e1 e2)) e1
+  | SndPair :
+    #e':closed_exp ->
+    #e'':closed_exp ->
+    hst:step e' e'' ->
+    step (ESnd e') (ESnd e'')
+  | SndPairReturn :
+    #e1:closed_exp ->
+    #e2:closed_exp ->
+    is_value (EPair e1 e2) ->
+    step (ESnd (EPair e1 e2)) e2
 
 let can_step (e:closed_exp) : Type0 =
-  Some? (step e)
+  exists (e':closed_exp). step e e'
 
 let irred (e:closed_exp) : Type0 =
-  None? (step e)
+  forall (e':closed_exp). ~(step e e') // optionally \/ is_value e - Amal's definition
 
 let rec lem_value_is_irred (e:closed_exp) : Lemma
   (requires is_value e)
   (ensures irred e)
   [SMTPat (irred e)] =
   match e with
-  | EPair e1 e2 -> lem_value_is_irred e1; lem_value_is_irred e2
+  | EUnit ->
+    assert (forall e'. ~(step EUnit e')) by explode ()
+  | ETrue ->
+    assert (forall e'. ~(step ETrue e')) by explode ()
+  | EFalse ->
+    assert (forall e'. ~(step EFalse e')) by explode ()
+  | ELam e11 ->
+    assert (forall e'. ~(step (ELam e11) e')) by explode ()
+  | EPair e1 e2 ->
+    lem_value_is_irred e1;
+    lem_value_is_irred e2;
+    introduce forall (e':closed_exp). step e e' ==> False with begin
+      introduce step e e' ==> False with h. begin
+        FStar.Squash.bind_squash #(step e e') () (fun st ->
+        match st with
+        | PairLeft e2 hst -> ()
+        | PairRight e1 is_val_e1 hst -> ()
+        | _ -> ())
+      end
+    end
   | _ -> ()
 
 (** reflexive transitive closure of step *)
+noeq
 type steps : closed_exp -> closed_exp -> Type =
 | SRefl  : e:closed_exp ->
            steps e e
-| STrans : #e:closed_exp ->
-           #e':closed_exp ->
-           squash (Some? (step e)) ->
-           steps (Some?.v (step e)) e' ->
-           steps e e'
+| STrans : #e1:closed_exp ->
+           #e2:closed_exp ->
+           #e3:closed_exp ->
+           step e1 e2 ->
+           steps e2 e3 ->
+           steps e1 e3
 
 let rec lem_steps_transitive_constructive
   (#e1 #e2 #e3:closed_exp)
@@ -316,16 +347,20 @@ let rec lem_steps_transitive_constructive
   = match st12 with
     | SRefl _ -> st23
     | STrans e1_can_step st12' ->
-      let e1' = Some?.v (step e1) in
       STrans e1_can_step (lem_steps_transitive_constructive st12' st23)
 
 open FStar.Squash
 
-let lem_step_implies_steps (e:closed_exp) :
+let lem_step_implies_steps (e e':closed_exp) :
   Lemma
-    (requires (Some? (step e)))
-    (ensures (steps e (Some?.v (step e)))) =
-  return_squash (STrans () (SRefl (Some?.v (step e))))
+    (requires step e e')
+    (ensures steps e e') =
+  introduce forall e e'. step e e' ==> steps e e' with begin
+    introduce step e e' ==> steps e e' with h. begin
+      FStar.Squash.bind_squash #(step e e') () (fun st ->
+        return_squash (STrans st (SRefl e')))
+    end
+  end
 
 let lem_steps_transitive (e1 e2 e3:closed_exp) :
   Lemma
@@ -395,8 +430,8 @@ let srefl_eapp_impossible (e1 e2 e':closed_exp) (st:steps (EApp e1 e2) e') (t1 t
     sem_expr_shape (TArr t1 t2) e1 /\
     (EApp e1 e2) == e')
   (ensures ~(irred e') \/ ~(sem_expr_shape (TArr t1 t2) e1))
-  =
-  match step e1 with
+  = admit ()
+  (*match step e1 with
   | Some e1' -> ()
   | None ->
     match step e2 with
@@ -404,15 +439,7 @@ let srefl_eapp_impossible (e1 e2 e':closed_exp) (st:steps (EApp e1 e2) e') (t1 t
     | None ->
       match e1 with
       | ELam e11 -> ()
-      | _ -> ()
-
-let e1_not_lam_impossible (e1:closed_exp) (t1:typ) (t2:typ) : Lemma
-  (requires
-    sem_expr_shape (TArr t1 t2) e1 /\
-    irred e1 /\
-    ~(ELam? e1))
-  (ensures ~(sem_expr_shape (TArr t1 t2) e1))
-  = ()
+      | _ -> ()*)
 
 (** Such a lemma is mentioned by Amal Ahmed in her PhD thesis, section 2
 
@@ -454,48 +481,41 @@ let rec destruct_steps_eapp
       steps (EApp e1 e2) (subst_beta e2' e11) /\
       steps (subst_beta e2' e11) e')
     (decreases st)
-  =
-  match st with
-  | SRefl (EApp e1 e2) ->
-    assert ((EApp e1 e2) == e');
-    srefl_eapp_impossible e1 e2 e' st t1 t2;
-    false_elim ()
-  | STrans e_can_step st' -> begin
-    match step e1 with
-    | Some e1' ->
-      let (EApp e1' e2) = Some?.v (step (EApp e1 e2)) in
-      lem_step_implies_steps e1;
-      lem_step_implies_steps (EApp e1 e2);
-      lem_steps_preserve_safe e1 e1';
-      lem_steps_preserve_sem_expr_shape e1 e1' (TArr t1 t2);
-      let s2 : steps (EApp e1' e2) e' = st' in
-      let (e11'', e2'') = destruct_steps_eapp e1' e2 e' s2 t1 t2 in
-      lem_steps_transitive e1 e1' (ELam e11'');
-      lem_steps_transitive (EApp e1 e2) (EApp e1' e2) (subst_beta e2'' e11'');
-      (e11'', e2'')
-    | None -> begin
-      match step e2 with
-      | Some e2' ->
-        let (EApp e1 e2') = Some?.v (step (EApp e1 e2)) in
-        lem_step_implies_steps e2;
-        lem_step_implies_steps (EApp e1 e2);
+  = match st with
+    | SRefl (EApp e1 e2) -> admit ()
+    | STrans #f1 #f2 #f3 step_eapp step_eapp_steps -> begin
+      let (EApp e1 e2) = f1 in
+      let e' = f3 in
+      match step_eapp with
+      | AppLeft #e1 e2 #e1' step_e1 -> begin
+        let (EApp e1' e2) = f2 in
+        lem_step_implies_steps e1 e1';
+        lem_step_implies_steps (EApp e1 e2) (EApp e1' e2);
+        lem_steps_preserve_safe e1 e1';
+        lem_steps_preserve_sem_expr_shape e1 e1' (TArr t1 t2);
+        let s2 : steps (EApp e1' e2) e' = step_eapp_steps in
+        let (e11'', e2'') = destruct_steps_eapp e1' e2 e' s2 t1 t2 in
+        lem_steps_transitive e1 e1' (ELam e11'');
+        lem_steps_transitive (EApp e1 e2) (EApp e1' e2) (subst_beta e2'' e11'');
+        (e11'', e2'')
+        end
+      | AppRight e1 #e2 #e2' is_val_e1 step_e2 -> begin
+        let (EApp e1 e2') = f2 in
+        lem_step_implies_steps e2 e2';
+        lem_step_implies_steps (EApp e1 e2) (EApp e1 e2');
         lem_steps_preserve_safe e2 e2';
-        let s2 : steps (EApp e1 e2') e' = st' in
+        let s2 : steps (EApp e1 e2') e' = step_eapp_steps in
         let (e11'', e2'') = destruct_steps_eapp e1 e2' e' s2 t1 t2 in
         lem_steps_transitive e2 e2' e2'';
         lem_steps_transitive (EApp e1 e2) (EApp e1 e2') (subst_beta e2'' e11'');
         (e11'', e2'')
-      | None -> begin
-        match e1 with
-        | ELam e11 ->
-          lem_step_implies_steps (EApp e1 e2);
-          (e11, e2)
-        | _ ->
-          e1_not_lam_impossible e1 t1 t2;
-          false_elim ()
         end
-    end
-  end
+      | Beta e11 e2 -> begin
+        lem_step_implies_steps (EApp e1 e2) (subst_beta e2 e11);
+        (e11, e2)
+        end
+      | _ -> false_elim ()
+      end
 
 let srefl_eif_impossible (e1 e2 e3 e':closed_exp) (st:steps (EIf e1 e2 e3) e') : Lemma
   (requires
@@ -505,22 +525,14 @@ let srefl_eif_impossible (e1 e2 e3 e':closed_exp) (st:steps (EIf e1 e2 e3) e') :
     sem_expr_shape TBool e1 /\
     (EIf e1 e2 e3) == e')
   (ensures ~(irred e') \/ ~(sem_expr_shape TBool e1))
-  =
-  match step e1 with
+  = admit ()
+  (*match step e1 with
   | Some e1' -> ()
   | None ->
     match e1 with
     | ETrue -> ()
     | EFalse -> ()
-    | _ -> ()
-
-let e1_not_bool_impossible (e1:closed_exp) : Lemma
-  (requires
-    sem_expr_shape TBool e1 /\
-    irred e1 /\
-    ~(ETrue? e1 \/ EFalse? e1))
-  (ensures  ~(sem_expr_shape TBool e1))
-  = ()
+    | _ -> ()*)
 
 let rec destruct_steps_eif
   (e1:closed_exp)
@@ -539,33 +551,37 @@ let rec destruct_steps_eif
       (ETrue? e1' ==> steps e2 e') /\
       (EFalse? e1' ==> steps e3 e'))
     (decreases st)
-  =
-  match st with
-  | SRefl (EIf e1 e2 e3) ->
-    let impossible : False = srefl_eif_impossible e1 e2 e3 e' st in false_elim impossible
-  | STrans e_can_step st' ->
-    match step e1 with
-    | Some e1' ->
-      let (EIf e1' e2 e3) = Some?.v (step (EIf e1 e2 e3)) in
-      lem_step_implies_steps e1;
-      lem_step_implies_steps (EIf e1 e2 e3);
-      lem_steps_preserve_safe e1 e1';
-      lem_steps_preserve_sem_expr_shape e1 e1' TBool;
-      let s2 : steps (EIf e1' e2 e3) e' = st' in
-      let e1'' = destruct_steps_eif e1' e2 e3 e' s2 in
-      lem_steps_transitive e1 e1' e1'';
-      lem_steps_transitive (EIf e1 e2 e3) (EIf e1' e2 e3) (EIf e1'' e2 e3);
-      e1''
-    | None ->
-      match e1 with
-      | ETrue ->
-        lem_step_implies_steps (EIf e1 e2 e3);
+  = match st with
+    | SRefl (EIf e1 e2 e3) -> begin
+      assert ((EIf e1 e2 e3) == e');
+      admit ()
+      end
+    | STrans #f1 #f2 #f3 step_eif step_eif_steps -> begin
+      let (EIf e1 e2 e3) = f1 in
+      let e' = f3 in
+      match step_eif with
+      | IfCond #e1 e2 e3 #e1' step_e1 -> begin
+        let (EIf e1' e2 e3) = f2 in
+        lem_step_implies_steps e1 e1';
+        lem_step_implies_steps (EIf e1 e2 e3) (EIf e1' e2 e3);
+        lem_steps_preserve_safe e1 e1';
+        lem_steps_preserve_sem_expr_shape e1 e1' TBool;
+        let s2 : steps (EIf e1' e2 e3) e' = step_eif_steps in
+        let e1'' = destruct_steps_eif e1' e2 e3 e' s2 in
+        lem_steps_transitive e1 e1' e1'';
+        lem_steps_transitive (EIf e1 e2 e3) (EIf e1' e2 e3) (EIf e1'' e2 e3);
+        e1''
+        end
+      | IfTrue e2 e3 -> begin
+        lem_step_implies_steps (EIf e1 e2 e3) e2;
         e1
-      | EFalse ->
-        lem_step_implies_steps (EIf e1 e2 e3);
+        end
+      | IfFalse e2 e3 -> begin
+        lem_step_implies_steps (EIf e1 e2 e3) e3;
         e1
-      | _ ->
-        let impossible : False = e1_not_bool_impossible e1 in false_elim impossible
+        end
+      | _ -> false_elim ()
+      end
 
   (**
     How the steps look like:
@@ -589,33 +605,38 @@ let rec destruct_steps_epair
       steps (EPair e1' e2') e')
     (decreases st)
   = match st with
-    | SRefl e -> (e1, e2)
-    | STrans e_can_step st' ->
-      match step e1 with
-      | Some e1' ->
-        let (EPair e1' e2) = Some?.v (step (EPair e1 e2)) in
-        lem_step_implies_steps e1;
-        lem_step_implies_steps (EPair e1 e2);
+    | SRefl (EPair e1 e2) -> begin
+      assume (is_value e1 /\ is_value e2);
+      (e1, e2)
+      end
+    | STrans #f1 #f2 #f3 step_epair step_epair_steps -> begin
+      let (EPair e1 e2) = f1 in
+      let e' = f3 in
+      match step_epair with
+      | PairLeft #e1 e2 #e1' step_e1 -> begin
+        let (EPair e1' e2) = f2 in
+        lem_step_implies_steps e1 e1';
+        lem_step_implies_steps (EPair e1 e2) (EPair e1' e2);
         lem_steps_preserve_safe e1 e1';
-        let s2 : steps (EPair e1' e2) e' = st' in
+        let s2 : steps (EPair e1' e2) e' = step_epair_steps in
         let (e1'', e2'') = destruct_steps_epair e1' e2 e' s2 in
         lem_steps_transitive e1 e1' e1'';
         lem_steps_transitive (EPair e1 e2) (EPair e1' e2) (EPair e1'' e2'');
         (e1'', e2'')
-      | None ->
-        match step e2 with
-        | Some e2' ->
-          let (EPair e1 e2') = Some?.v (step (EPair e1 e2)) in
-          lem_step_implies_steps e2;
-          lem_step_implies_steps (EPair e1 e2);
-          lem_steps_preserve_safe e2 e2';
-          let s2 : steps (EPair e1 e2') e' = st' in
-          let (e1'', e2'') = destruct_steps_epair e1 e2' e' s2 in
-          lem_steps_transitive e2 e2' e2'';
-          lem_steps_transitive (EPair e1 e2) (EPair e1 e2') (EPair e1'' e2'');
-          (e1'', e2'')
-        | None ->
-          (e1, e2)
+        end
+      | PairRight e1 #e2 #e2' is_val_e1 step_e2 -> begin
+        let (EPair e1 e2') = f2 in
+        lem_step_implies_steps e2 e2';
+        lem_step_implies_steps (EPair e1 e2) (EPair e1 e2');
+        lem_steps_preserve_safe e2 e2';
+        let s2 : steps (EPair e1 e2') e' = step_epair_steps in
+        let (e1'', e2'') = destruct_steps_epair e1 e2' e' s2 in
+        lem_steps_transitive e2 e2' e2'';
+        lem_steps_transitive (EPair e1 e2) (EPair e1 e2') (EPair e1'' e2'');
+        (e1'', e2'')
+        end
+      | _ -> (e1, e2)
+      end
 
   (**
     How the steps look like:
@@ -642,32 +663,32 @@ let rec destruct_steps_epair_fst
     (ensures fun e12' ->
       irred e12' /\
       steps e12 e12' /\
+      is_closed (EFst e12') /\
       steps (EFst e12') e')
     (decreases st)
   =
   match st with
-  | SRefl (EFst e12) -> false_elim ()
-  | STrans e_can_step st' -> begin
-    match step e12 with
-    | Some e12' -> begin
-      let (EFst e12') = Some?.v (step (EFst e12)) in
-      lem_step_implies_steps e12;
-      lem_step_implies_steps (EFst e12);
+  | SRefl (EFst e12) -> admit ()
+  | STrans #f1 #f2 #f3 step_efst step_efst_steps -> begin
+    let (EFst e12) = f1 in
+    let e' = f3 in
+    match step_efst with
+    | FstPair #e12 #e12' step_e12 -> begin
+      let (EFst e12') = f2 in
+      lem_step_implies_steps e12 e12';
+      lem_step_implies_steps (EFst e12) (EFst e12');
       lem_steps_preserve_safe e12 e12';
       lem_steps_preserve_sem_expr_shape e12 e12' (TPair t1 t2);
-      let s2 : steps (EFst e12') e' = st' in
+      let s2 : steps (EFst e12') e' = step_efst_steps in
       let e12'' = destruct_steps_epair_fst e12' e' s2 t1 t2 in
       lem_steps_transitive e12 e12' e12'';
       e12''
       end
-    | None -> begin
-      match e12 with
-      | EPair e1 _ -> begin
-        lem_step_implies_steps (EFst e12);
-        e12
-        end
-      | _ -> false_elim ()
+    | FstPairReturn #e1 #e2 is_val_epair -> begin
+      lem_step_implies_steps (EFst (EPair e1 e2)) e1;
+      e12
       end
+    | _ -> false_elim ()
     end
 
   (**
@@ -694,32 +715,32 @@ let rec destruct_steps_epair_snd
     (ensures fun e12' ->
       irred e12' /\
       steps e12 e12' /\
+      is_closed (ESnd e12') /\
       steps (ESnd e12') e')
     (decreases st)
   =
   match st with
-  | SRefl (ESnd e12) -> false_elim ()
-  | STrans e_can_step st' -> begin
-    match step e12 with
-    | Some e12' -> begin
-      let (ESnd e12') = Some?.v (step (ESnd e12)) in
-      lem_step_implies_steps e12;
-      lem_step_implies_steps (ESnd e12);
+  | SRefl (ESnd e12) -> admit ()
+  | STrans #f1 #f2 #f3 step_esnd step_esnd_steps -> begin
+    let (ESnd e12) = f1 in
+    let e' = f3 in
+    match step_esnd with
+    | SndPair #e12 #e12' step_e12 -> begin
+      let (ESnd e12') = f2 in
+      lem_step_implies_steps e12 e12';
+      lem_step_implies_steps (ESnd e12) (ESnd e12');
       lem_steps_preserve_safe e12 e12';
       lem_steps_preserve_sem_expr_shape e12 e12' (TPair t1 t2);
-      let s2 : steps (ESnd e12') e' = st' in
+      let s2 : steps (ESnd e12') e' = step_esnd_steps in
       let e12'' = destruct_steps_epair_snd e12' e' s2 t1 t2 in
       lem_steps_transitive e12 e12' e12'';
       e12''
       end
-    | None -> begin
-      match e12 with
-      | EPair _ e2 -> begin
-        lem_step_implies_steps (ESnd e12);
-        e12
-        end
-      | _ -> false_elim ()
+    | SndPairReturn #e1 #e2 is_val_epair -> begin
+      lem_step_implies_steps (ESnd (EPair e1 e2)) e2;
+      e12
       end
+    | _ -> false_elim ()
     end
 
   (**
